pulse/examples/dsls/mini_steel/Pulse.Checker.fsti
@@ -8,10 +8,24 @@ open Pulse.Syntax
 open Pulse.Elaborate.Pure
 open Pulse.Typing
 
+val readback_universes (us:list R.universe)
+  : o:option (list universe) { 
+          Some? o ==> List.Tot.map elab_universe (Some?.v o) == us 
+    }
+
+val readback_qual (q:R.aqualv)
+  : option qualifier
+  
+val readback_ty (t:R.term)
+  : T.Tac (option (ty:pure_term { elab_term ty == Some t }))
+
+val readback_comp (t:R.term)
+  : T.Tac (option (c:comp{ elab_comp c == Some t}))
+
 val check_tot (f:RT.fstar_top_env) (g:env) (t:term)
   : T.Tac (_:(ty:pure_term &
               src_typing f g t (C_Tot ty)) { is_pure_term t })
-
+  
 type check_t =
   f:RT.fstar_top_env ->
   g:env ->
